src/covering.mli
@@ -51,16 +51,16 @@ val pat_of_constr : constr -> pat
 val pr_constr_pat : env -> constr -> Pp.std_ppcmds
 val pr_pat : env -> pat -> Pp.std_ppcmds
 val pr_context : env -> rel_context -> Pp.std_ppcmds
-val ppcontext : rel_context -> unit
+val ppcontext : env -> rel_context -> unit
 val pr_context_map : env -> context_map -> Pp.std_ppcmds
-val ppcontext_map : context_map -> unit
+val ppcontext_map : env -> context_map -> unit
 val typecheck_map :
-  Evd.evar_map -> context_map -> unit
+  env -> Evd.evar_map -> context_map -> unit
 val check_ctx_map :
-  Evd.evar_map -> context_map -> context_map
+  env -> Evd.evar_map -> context_map -> context_map
 
 (** Smart constructor (doing runtime checks) *)
-val mk_ctx_map :
+val mk_ctx_map : Environ.env ->
   Evd.evar_map ->
   rel_context ->
   pat list ->
@@ -84,7 +84,7 @@ val subst_constr_pat : int -> constr -> pat -> pat
 val subst_constr_pats : int -> constr -> pat list -> pat list
 val subst_rel_context :
   int ->
-  constr ->
+  constr list ->
   rel_context ->
   rel_context
 val subst_telescope :
@@ -107,7 +107,7 @@ val lift_pats : int -> pat list -> pat list
 type path = Evd.evar list
 
 type splitting =
-    Compute of context_map * types * splitting_rhs
+    Compute of context_map * where_clause list * types * splitting_rhs
   | Split of context_map * int * types * splitting option array
   | Valid of context_map * types * identifier list *
       Tacmach.tactic * (Proofview.entry * Proofview.proofview) *
@@ -115,6 +115,9 @@ type splitting =
   | Mapping of context_map * splitting
   | RecValid of identifier * splitting
   | Refined of context_map * refined_node * splitting
+
+and where_clause =  
+  identifier * named_context * context_map * constr * types * splitting
 
 and refined_node = {
   refined_obj : identifier * constr * types;
@@ -135,7 +138,7 @@ val pr_path : Evd.evar_map -> Evd.evar list -> Pp.std_ppcmds
 val eq_path : Evar.t list -> Evar.t list -> bool
 
 val pr_splitting : env -> splitting -> Pp.std_ppcmds
-val ppsplit : splitting -> unit
+val ppsplit : env -> splitting -> unit
 
 (** Covering computation *)
 
@@ -187,7 +190,7 @@ val check_eq_context_nolet :
   Evd.evar_map ->
   context_map ->
   context_map -> unit
-val compose_subst :
+val compose_subst : Environ.env ->
   ?sigma:Evd.evar_map ->
   context_map ->
   context_map ->
@@ -197,7 +200,7 @@ val push_mapping_context :
   context_map ->
   context_map
 val lift_subst :
-  Evd.evar_map -> context_map -> rel_context -> context_map
+  Environ.env -> Evd.evar_map -> context_map -> rel_context -> context_map
 val single_subst :
   env ->
   Evd.evar_map ->
@@ -322,6 +325,15 @@ val rel_id : (Name.t * 'a * 'b) list -> int -> Id.t
 val push_named_context :
   named_context -> env -> env
 
+val env_of_rhs : 
+           Evd.evar_map ref ->
+           Context.rel_context ->
+           Environ.env ->
+           (Names.Id.t * pat) list ->
+           Context.rel_declaration list ->
+           (Names.name * Constr.constr option * Constr.constr) list *
+           Environ.env * int * Constr.constr list
+
 val covering_aux :
   env ->
   Evd.evar_map ref ->
@@ -336,6 +348,6 @@ val covering :
   env ->
   Evd.evar_map ref ->
   identifier * bool * Constrintern.internalization_env ->
-  clause list ->
+  clause list -> Evd.evar list ->
   context_map ->
   constr -> splitting
